ind_cpa: split aenc into separate function, finish proof other than public_rel_elem/double_squiggle stuff

examples/ind_cpa.v
@@ -11,7 +11,7 @@ From cryptis.primitives Require Import attacker.
 From reloc Require Import reloc.
 From cryptis Require Import lib_spec.
 From cryptis.core Require Import minted_spec term_meta_spec rel.
-From cryptis.primitives Require Import simple_spec with_cryptis_spec.
+From cryptis.primitives Require Import simple_spec comp_spec with_cryptis_spec.
 
 Set Implicit Arguments.
 Unset Strict Implicit.
@@ -34,19 +34,54 @@ Variable N : namespace.
 A --> *: if b then {nonce, msg_0}@pkA else {nonce, msg_1}@pkA
 
 *)
+
+Definition aenc' : val := λ: "pk" "m",
+  let: "nonce" := mk_nonce #() in
+  aenc "pk" (Tag $ N.@"m") (term_of_list ["nonce"; "m"]).
+
 Definition alice : val := λ: "c",
   let: "skA" := mk_aenc_key #() in
   let: "pkA" := pkey "skA" in
   send "c" "pkA";;
-  let: "nonce" := mk_nonce #() in
   let: "msg_0" := recv "c" in
   let: "msg_1" := recv "c" in
   let: "b" := nondet_bool #() in
   let: "msg" := if: "b" then "msg_0" else "msg_1" in
-  send "c" (aenc "pkA" (Tag $ N.@"m") (term_of_list ["nonce"; "msg"]));;
-  let: "b'" := recv "c" in
-  let: "b'" := eq_term (TInt 1) "b'" in
-  ("b", "b'").
+  send "c" (aenc' "pkA" "msg");;
+  let: "guess" := recv "c" in
+  let: "guess" := eq_term (TInt 1) "guess" in
+  ("b", "guess").
+
+Lemma rel_aenc' (sk sk' : aenc_key) (m m' : term) (Ψ : val → val → iProp) :
+  cryptis_rel_ctx -∗
+  minted (Spec.pkey sk) -∗ minted_spec (Spec.pkey sk') -∗
+  minted m -∗ minted_spec m' -∗
+  (∀ c c', publicly_related c c' -∗ Ψ c c') -∗
+  REL aenc' (Spec.pkey sk) m << aenc' (Spec.pkey sk') m' : Ψ.
+Proof.
+iIntros "#Hctx #mintsk #mint_specsk' #mintm #mint_specm' post". rewrite /aenc'.
+rel_pures_l. rel_pures_r.
+rel_apply_l (rel_mk_nonce_l _ _ (λ _, ∅) with "[//]").
+{ iIntros "%t". by iApply big_sepS_empty. }
+iIntros (nonce) "%Hnonce #mint_nonce _".
+rel_apply_r (rel_mk_nonce_r _ _ (λ _, ∅) with "[//]").
+{ iIntros "%t". by iApply big_sepS_empty. }
+iIntros (nonce') "%Hnonce' #mint_spec_nonce' _".
+rel_pures_l. rel_pures_r.
+rel_apply_l rel_nil_l.
+repeat rel_apply_l rel_cons_l. rel_apply_l rel_term_of_list_l.
+rel_apply_r rel_nil_r.
+repeat rel_apply_r rel_cons_r. rel_apply_r rel_term_of_list_r.
+rel_apply_l rel_aenc_l.
+iIntros (cmsg) "%Hcmsg".
+rel_apply_r rel_aenc_r.
+iIntros (cmsg') "%Hcmsg'".
+rel_values. iApply "post".
+rewrite Hcmsg Hcmsg' publicly_related_aenc.
+iRight.
+rewrite minted_of_list minted_spec_of_list=> /=.
+iFrame "#".
+Admitted.
 
 Lemma rel_alice c c' (b: bool) :
   cryptis_rel_ctx -∗
@@ -67,51 +102,58 @@ rel_apply_l rel_pkey_l. rel_apply_r rel_pkey_r.
 rel_pures_l. rel_pures_r.
 iAssert (|={⊤}=> publicly_related (Spec.pkey skA) (Spec.pkey skA'))%I
           with "[token_skA token_spec_skA']" as ">#Hpub".
-{ iApply publicly_related_aenc_key_pkey. iLeft.
-  iApply publicly_related_aenc_key_seed. admit. }
+{ iApply publicly_related_aenc_key_pkey. iRight.
+  iFrame "#".
+  admit. }
 rel_bind_l (send _ _). rel_bind_r (send _ _).
-iApply (refines_bind _ _ _ lrel_unit); first by iApply rel_send.
+iApply refines_bind; first by iApply rel_send.
 iIntros (? ?) "[-> ->]"=> /=.
 rel_pures_l. rel_pures_r.
-rel_apply_l (rel_mk_nonce_l _ _ (λ _, ∅) with "[//]").
-{ iIntros "%t". by iApply big_sepS_empty. }
-iIntros (nonce) "%Hnonce #mint_nonce _".
-rel_apply_r (rel_mk_nonce_r _ _ (λ _, ∅) with "[//]").
-{ iIntros "%t". by iApply big_sepS_empty. }
-iIntros (nonce') "%Hnonce' #mint_spec_nonce' _".
+rel_bind_l (recv _). rel_bind_r (recv _).
+iApply refines_bind'. iApply rel_recv=> //.
+iIntros (msg_0 msg_0') "#Hmsg_0"=> /=.
 rel_pures_l. rel_pures_r.
 rel_bind_l (recv _). rel_bind_r (recv _).
-iApply (refines_bind _ _ _ (λ v v', ∃ t t', ⌜v = t ∧ v' = t'⌝ ∧ publicly_related t t')%I);
-  first by iApply (rel_recv with "[//]"); eauto.
-iIntros (? ?) "(%msg_0 & %msg_0' & [-> ->] & #Hmsg_0)"=> /=.
+iApply refines_bind'. iApply rel_recv=> //.
+iIntros (msg_1 msg_1') "#Hmsg_1"=> /=.
+rel_pures_l. rel_pures_r.
+rel_apply_l rel_nondet_bool_l. iIntros (choice); rel_pures_l.
+rel_apply_r (rel_nondet_bool_r _ _ (negb choice)); rel_pures_r.
+rel_bind_l (if: _ then _ else _)%E.
+rel_bind_r (if: _ then _ else _)%E.
+iApply (refines_bind _ _ _ (λ v v', ∃ m m' : term, ⌜v = m⌝ ∧ ⌜v' = m'⌝ ∧ minted m ∧ minted_spec m')%I).
+{ rewrite (publicly_related_minted msg_0) (publicly_related_minted msg_1).
+  iDestruct "Hmsg_0" as "[? ?]".
+  iDestruct "Hmsg_1" as "[? ?]".
+  case: choice; rel_pures_l; rel_pures_r; rel_values.
+  iExists msg_0, msg_1'; iFrame "#"; eauto.
+  iExists msg_1, msg_0'; iFrame "#"; eauto. }
+iIntros (? ?) "(%msg & %msg' & -> & -> & #mint_msg & #mint_spec_msg')"=> /=.
+rel_pures_l. rel_pures_r.
+rel_bind_l (aenc' _ _). rel_bind_r (aenc' _ _).
+iApply refines_bind'. iApply rel_aenc'=> //=.
+by rewrite minted_pkey. by rewrite minted_spec_pkey.
+rewrite (publicly_related_minted msg_0).
+iIntros (c_msg c_msg') "#Hcmsg".
+rel_bind_l (send _ _). rel_bind_r (send _ _).
+iApply refines_bind; first by iApply rel_send.
+iIntros (? ?) "[-> ->]"=> /=.
 rel_pures_l. rel_pures_r.
 rel_bind_l (recv _). rel_bind_r (recv _).
-iApply (refines_bind _ _ _ (λ v v', ∃ t t', ⌜v = t ∧ v' = t'⌝ ∧ publicly_related t t')%I);
-  first by iApply (rel_recv with "[//]"); eauto.
-iIntros (? ?) "(%msg_1 & %msg_1' & [-> ->] & #Hmsg_1)"=> /=.
+iApply refines_bind'. iApply rel_recv=> //.
+iIntros (guess guess') "#Hguess"=> /=.
 rel_pures_l. rel_pures_r.
-rel_apply_l rel_nondet_bool_l. iIntros ([]).
-- rel_apply_r (rel_nondet_bool_r _ _ false).
-  rel_pures_l. rel_pures_r.
-  set K := [AppRCtx (send c);
-  AppRCtx
-  (λ: <>,
-  let: "b'" := recv c in
-  let: "b'" := eq_term (TInt 1) "b'" in (#true, "b'"))].
-  set e := (send c'
-  (aenc (Spec.pkey skA') (Tag (N.@"m"))
-  (term_of_list (nonce' :: msg_1' :: InjLV #())));;
-  let: "b'" := recv c' in let: "b'" := eq_term (TInt 1) "b'" in
-  (#false, "b'"))%E.
-  set Ψ := (λ p1 p2 : val,
-  ⌜∃ b1 b'1 b2 b'2 : bool,
-  p1 = (#b1, #b'1)%V ∧ p2 = (#b2, #b'2)%V ∧ (b = b1
-  → b ≠ b2 ∧ b'1 = b'2)⌝)%I.
-  set t := (term_of_list (nonce :: msg_0 :: InjLV #())%E).
-  (* rel_apply_l rel_term_of_list_l. ?? *)
-  rel_apply_l (rel_aenc_l ⊤ K e skA (N.@"m") _ Ψ).
-  admit.
-- rel_apply_r (rel_nondet_bool_r _ _ true).
-  rel_pures_l. rel_pures_r.
-  admit.
+rel_bind_l (eq_term _ _). rel_bind_r (eq_term _ _).
+iApply refines_bind'. iApply rel_eq_term=> /=.
+rel_pures_l. rel_pures_r.
+rel_values.
+iAssert (▷ ⌜TInt 1 = guess ↔ TInt 1 = guess'⌝)%I as ">%H".
+{ iApply publicly_related_part_bij'=> //.
+  by rewrite publicly_related_TInt. }
+iPureIntro.
+eexists _, _, _, _. repeat split; eauto.
+destruct choice=> /=; congruence.
+by apply bool_decide_ext.
 Admitted.
+
+End CPA.
